proofchat/bin/client.mli
@@ -3,12 +3,7 @@ type nat =
 | O
 | S of nat
 
-type comparison =
-| Eq
-| Lt
-| Gt
-
-val compOpp : comparison -> comparison
+val app : 'a1 list -> 'a1 list -> 'a1 list
 
 type positive =
 | XI of positive
@@ -19,18 +14,9 @@ type n =
 | N0
 | Npos of positive
 
-type z =
-| Z0
-| Zpos of positive
-| Zneg of positive
-
 module Pos :
  sig
   val succ : positive -> positive
-
-  val compare_cont : comparison -> positive -> positive -> comparison
-
-  val compare : positive -> positive -> comparison
 
   val of_succ_nat : nat -> positive
  end
@@ -52,24 +38,45 @@ val ascii_of_N : n -> char
 
 val ascii_of_nat : nat -> char
 
-module Z :
- sig
-  val compare : z -> z -> comparison
 
-  val leb : z -> z -> bool
-
-  val of_nat : nat -> z
- end
-
-val length : string -> nat
 
 type 'x optionE =
 | SomeE of 'x
 | NoneE of string
 
+val add : Uint63.t -> Uint63.t -> Uint63.t
+
+val sub : Uint63.t -> Uint63.t -> Uint63.t
+
+val ltsb : Uint63.t -> Uint63.t -> bool
+
+val lesb : Uint63.t -> Uint63.t -> bool
+
+type bytes = char list
+
+val send :
+  Unix.file_descr -> bytes -> Uint63.t -> Uint63.t -> Unix.msg_flag list ->
+  Uint63.t
+
+val sub1_no_underflow : Uint63.t -> bool
+
 val space : char
 
 val no_spaces : string -> bool
+
+val string_of_socket_addr : Unix.sockaddr -> string
+
+val int_len_list : 'a1 list -> Uint63.t
+
+val bytes_of_string : string -> bytes
+
+val string_of_bytes : bytes -> string
+
+val int_len_string : string -> Uint63.t
+
+val create_list : 'a1 -> Uint63.t -> 'a1 list
+
+val pad_string_r : string -> char -> Uint63.t -> string
 
 type username =
   string
@@ -79,6 +86,21 @@ val validate_username : string -> bool
 
 val new_username : string -> username optionE
 
-val print_socket_addr : Unix.sockaddr -> unit
+type client_message =
+| REG of username
+| MESG of string
+| PMSG of string * username
+| EXIT of username
+
+val serialize_string : string -> bytes
+
+val serialize_username : username -> bytes
+
+val serialize_client_message : client_message -> bytes
+
+val resend :
+  Uint63.t -> Uint63.t -> Unix.file_descr -> bytes -> Uint63.t -> unit optionE
+
+val send_message : Unix.file_descr -> bytes -> unit optionE
 
 val client : string -> int -> unit optionE
