proofchat/bin/pfbytes.ml
@@ -1,0 +1,16 @@
+let bytes_of_byte_list (l : char list) : bytes =
+  Bytes.concat Bytes.empty (List.map (fun c -> Bytes.make 1 c) l)
+
+let int63_to_bytes n =
+  let bytes = Bytes.create 8 in
+  for i = 0 to 7 do
+    Bytes.set bytes i (Char.chr ((n lsr (i * 8)) land 0xFF))
+  done;
+  bytes
+
+let bytes_to_int63 bytes =
+  let n = ref 0 in
+  for i = 0 to 7 do
+    n := !n lor ((Char.code (Bytes.get bytes i)) lsl (i * 8))
+  done;
+  !n
