theories/StringTheory.v
@@ -3,8 +3,11 @@
     A collection of [string]-related definitions
 *)
 
+Require Export OCamlTypes.
 Require Export String.
 Require Export Ascii.
+Require Export List.
+Export ListNotations.
 Open Scope string.
 
 (**
@@ -41,3 +44,49 @@ Fixpoint no_spaces (s : string) : bool :=
         else
             no_spaces s'
     end.
+
+(**
+    Prints a sockaddr
+*)
+Definition string_of_socket_addr (s : sockaddr) : string :=
+    match s with
+    | ADDR_UNIX s' => s'
+    | ADDR_INET addr p =>
+        (string_of_inet_addr addr) ++ ":" ++ (string_of_int p)
+    end.
+
+
+(** OCaml int list length *)
+Fixpoint int_len_list {X : Type} (l : list X) : int :=
+    match l with
+    | [] => 0
+    | _ :: t => 1 + int_len_list t
+    end.
+
+Fixpoint bytes_of_string (s : string) : bytes :=
+    match s with
+    | EmptyString => [x00]
+    | String a s' => (byte_of_ascii a) :: bytes_of_string s'
+    end.
+
+Fixpoint string_of_bytes (b : bytes) : string :=
+    match b with
+    | [] | [x00] => EmptyString
+    | h :: t => String (ascii_of_byte h) (string_of_bytes t)
+    end.
+
+(** OCaml int string length *)
+Definition int_len_string (s : string) : int :=
+    int_len_list (bytes_of_string s).
+
+Function create_list {X : Type} (x : X) (n : int) 
+    {measure (fun x => (Z.to_nat (to_Z x))) n} : list X :=
+    (if sub1_no_underflow n then
+        x :: (create_list x (n - 1))
+    else
+        [])%sint63.
+    prove_sub1.
+Defined.
+
+Definition pad_string_r (s : string) (b : byte) (target_len : int) : string :=
+    s ++ (string_of_bytes (create_list byte b (target_len - int_len_string s + 1))). 
