theories/Client.v
@@ -5,76 +5,36 @@
 
 Require Import Messages.
 Require Import Monads.
-Require Import Program.
 Require Import Recdef.
 Open Scope monad_scope.
 
 (**
-    A helper lemma for below
-*)
-Lemma Z_lt_impl_nat_lt : forall z1 z2,
-    0 <= z1 < z2 ->
-    (Z.to_nat z1 < Z.to_nat z2)%nat.
-Proof.
-    intros. destruct H as [Z1Nonneg Z1Z2].
-    assert (0 <= z2). {
-        transitivity z1.
-            assumption.
-        now apply Z.lt_le_incl.
-    }
-    now apply Z2Nat.inj_lt.
-Qed.
-
-(**
-    Defines if an OCaml integer has underflown
-*)
-Definition no_underflow n : bool := 
-    n - 1 <? n.
-
-(**
     The internal loop of our client sending thread
 *)
-Function client_send_thread_internal (timeout : int)
-        {measure (fun x => (Z.to_nat (to_Z x))) timeout} : int :=
-    if ((0 <=? timeout - 1) && no_underflow timeout) then
-        1 + client_send_thread_internal (timeout - 1)
-    else
-        0.
-Proof.
-    intros.
-    unfold no_underflow in teq.
-    apply Bool.andb_true_iff in teq.
-    destruct teq as [Gt0 NoUnderflow].
-    apply Z_lt_impl_nat_lt. split.
-    - change 0%Z with (to_Z 0).
-        now apply leb_spec.
-    - now apply ltb_spec.
-Defined.
-
-(**
-    Prints a sockaddr
-*)
-Definition print_socket_addr (s : sockaddr) : unit :=
-    match s with
-    | ADDR_UNIX s' => print_string s'
-    | ADDR_INET addr p =>
-        let* _ <= print_string (string_of_inet_addr addr) #;
-        let* _ <= print_string ":" #;
-        print_int p
-    end.
+Definition client_send_thread_internal (_ : unit) : optionE unit :=
+    repeat_until_timeout max_int (fun _ => SomeE tt).
 
 (**
     Wraps up all client logic: port binding, threading, etc.
 *)
 Definition client (host : string) (portno : port) : optionE unit :=
+    (* Obtain username from user *)
     let* _ <= print_endline "Please enter a username (length 1-32, no spaces)" #;
     let username_string := read_line tt in
     uname <- new_username username_string ;;
+    (* Create a TCP socket to server *)
     let socket_fd := socket PF_INET SOCK_STREAM 0 in
     let socket_addr := ADDR_INET (inet_addr_of_string host) portno in
-    let* _ <= print_string "Opening client connection to " #;
-    let* _ <= print_socket_addr socket_addr #;
-    let* _ <= print_string " as " #;
-    let* _ <= print_socket_addr (getsockname socket_fd) #;
-    let* _ <= print_endline "" #;
+    let* _ <= print_endline ("Opening client connection to " ++ 
+        (string_of_socket_addr socket_addr) ++ " as " ++
+        (string_of_socket_addr (getsockname socket_fd))) #;
+    let* _ <= connect socket_fd socket_addr #;
+    (* Send REG message to server *)
+    _ <- send_message socket_fd (serialize_client_message (REG uname)) ;;
+    (* Receive ACK from server *)
+    (* Display chatroom information to user output *)
+    (* Wait for user input *)
+    (* Wait for chat messages from server *)
+    let* _ <= print_endline "Closing client connection" #;
+    let* _ <= close socket_fd #;
     return tt.
