theories/OCamlTypes.v
@@ -5,8 +5,13 @@
     user input, networking, and operating system behavior.
 *)
 
+Require Import Recdef.
+Require Import Monads.
+Open Scope monad_scope.
+
 (** Strings *)
-Require Export Ascii String.
+Require Export Ascii String Strings.Byte.
+Definition bytes := list byte.
 
 (** OCaml Integers *)
 Require Export Coq.Numbers.Cyclic.Int63.Sint63.
@@ -25,7 +30,67 @@ Axiom print_string : string -> unit.
 Axiom print_int : int -> unit.
 Axiom print_endline : string -> unit.
 Axiom socket : socket_domain -> socket_type -> int -> file_descr.
+Axiom connect : file_descr -> sockaddr -> unit.
+Axiom send : file_descr -> bytes -> int -> int -> list msg_flag -> int.
+Axiom close : file_descr -> unit.
+Axiom string_of_int : int -> string.
 Axiom sleep : int -> unit.
 Axiom inet_addr_of_string : string -> inet_addr.
 Axiom string_of_inet_addr : inet_addr -> string.
 Axiom getsockname : file_descr -> sockaddr.
+
+Axiom int63_to_bytes : int -> bytes.
+Axiom bytes_to_int63 : bytes -> int.
+
+
+(**
+    A helper lemma for below
+*)
+Lemma Z_lt_impl_nat_lt : forall (z1 z2 : Z),
+    (0 <= z1 < z2)%Z ->
+    (Z.to_nat z1 < Z.to_nat z2)%nat.
+Proof.
+    intros. destruct H as [Z1Nonneg Z1Z2].
+    assert (0 <= z2)%Z. {
+        transitivity z1.
+            assumption.
+        now apply Z.lt_le_incl.
+    }
+    now apply Z2Nat.inj_lt.
+Qed.
+
+(**
+    Defines if an OCaml integer has underflown
+*)
+Definition sub1_no_underflow (n : int) : bool := 
+    ((0 <=? n - 1) && (n - 1 <? n))%sint63.
+
+Ltac prove_sub1 :=
+    intros;
+    unfold sub1_no_underflow in *;
+    match goal with
+    [H: _ && _ = true |- _] => 
+        apply Bool.andb_true_iff in H;
+        destruct H as [Gt0 NoUnderflow];
+        apply Z_lt_impl_nat_lt; split; [
+        change 0%Z with (to_Z 0);
+            now apply leb_spec
+        | now apply ltb_spec
+        ]
+    end.
+
+(** 
+    Calls a function f until either it terminates with SomeE tt,
+    or timeout occurs
+*)
+Function repeat_until_timeout (timeout : int) (f : unit -> optionE unit)
+        {measure (fun x => (Z.to_nat (to_Z x))) timeout} : optionE unit :=
+    (if sub1_no_underflow timeout then
+        match f tt with
+        | SomeE x => SomeE x
+        | NoneE _ => repeat_until_timeout (timeout - 1) f
+        end
+    else
+        NoneE "Timeout occurred")%sint63.
+    prove_sub1.
+Defined.
