theories/PCExtract.v
@@ -4,8 +4,8 @@
 *)
 
 Require Extraction.
+Require Import StringTheory.
 Require Import Client.
-Require Import OCamlTypes.
 Require Import Monads.
 Require Import Sockets.
 Require Import ExtrOcamlBasic.
@@ -20,6 +20,7 @@ Extract Inlined Constant read_line => "read_line".
 Extract Inlined Constant print_int => "print_int".
 Extract Inlined Constant print_string => "print_string".
 Extract Inlined Constant print_endline => "print_endline".
+Extract Inlined Constant string_of_int => "string_of_int".
 Extract Inlined Constant socket => "Unix.socket".
 Extract Inlined Constant sleep => "Unix.sleep".
 Extract Inlined Constant inet_addr_of_string => "Unix.inet_addr_of_string".
@@ -27,6 +28,14 @@ Extract Inlined Constant string_of_inet_addr => "Unix.string_of_inet_addr".
 Extract Inlined Constant getsockname => "Unix.getsockname".
 Extract Inlined Constant inet_addr => "Unix.inet_addr".
 Extract Inlined Constant file_descr => "Unix.file_descr".
+Extract Inlined Constant connect => "Unix.connect".
+Extract Constant send => "(fun a b c d e -> Unix.send a (Pfbytes.bytes_of_byte_list b) c d e)".
+Extract Inlined Constant close => "Unix.close".
+Extract Inlined Constant int63_to_bytes => "Pfbytes.int63_to_bytes".
+Extract Inlined Constant bytes_to_int63 => "Pfbytes.bytes_to_int63".
+
+(* Extract Inlined Constant int_len_list => "Bytes.length".
+Extract Inlined Constant bytes_of_string => "Bytes.of_string". *)
 
 Extract Inlined Constant port => "int".
 Extract Inductive socket_domain => 
@@ -35,6 +44,8 @@ Extract Inductive socket_type =>
     "Unix.socket_type" [ "Unix.SOCK_STREAM" "Unix.SOCK_DGRAM" "Unix.SOCK_RAW" "Unix.SOCK_SEQPACKET" ].
 Extract Inductive sockaddr =>
     "Unix.sockaddr" [ "Unix.ADDR_UNIX" "Unix.ADDR_INET" ].
+Extract Inductive msg_flag =>
+    "Unix.msg_flag" [ "Unix.MSG_OOB" "Unix.MSG_DONTROUTE" "Unix.MSG_PEEK" ].
 
 Recursive Extraction client.
 Extraction "client.ml" client.
