theories/Communication.v
@@ -1,0 +1,6 @@
+(** * Communication
+
+    Routines for sending messages
+*)
+
+
